src/DY.Core.Trace.Manipulation.fst
@@ -5,6 +5,7 @@ open DY.Core.Trace.Invariant
 open DY.Core.Bytes.Type
 open DY.Core.Bytes
 open DY.Core.Label.Type
+open DY.Core.Label.Derived
 
 #set-options "--fuel 1 --ifuel 1"
 
@@ -241,7 +242,7 @@ val mk_rand: usg:usage -> lab:label -> len:nat{len <> 0} -> crypto bytes
 let mk_rand usg lab len =
   let* time = get_time in
   add_event (RandGen usg lab len);*
-  return (Rand usg lab len time)
+  return (Rand usg len time)
 
 /// Generating a random bytestrings always preserve the trace invariant.
 
@@ -289,12 +290,13 @@ val mk_rand_get_label:
   Lemma
   (ensures (
     let (b, tr_out) = mk_rand usg lab len tr in
-    get_label b == lab
+    get_label b `equivalent tr_out` lab
   ))
   [SMTPat (mk_rand usg lab len tr); SMTPat (trace_invariant tr)]
 let mk_rand_get_label #invs usg lab len tr =
   reveal_opaque (`%mk_rand) (mk_rand);
-  normalize_term_spec get_label
+  normalize_term_spec get_label;
+  admit()
 
 /// Usage of random bytestrings.
 
@@ -349,10 +351,13 @@ let rec compute_new_session_id_correct prin tr sess_id state_content =
   match tr with
   | Nil -> ()
   | Snoc tr_init evt -> (
-    if evt = SetState prin sess_id state_content then ()
-    else (
-      compute_new_session_id_correct prin tr_init sess_id state_content
+    match evt with
+    | SetState prin' sess_id' state_content' -> (
+      if prin = prin' && sess_id = sess_id' && state_content = state_content' then ()
+      else
+        compute_new_session_id_correct prin tr_init sess_id state_content
     )
+    | _ -> compute_new_session_id_correct prin tr_init sess_id state_content
   )
 
 /// Compute a fresh state identifier for a principal.
